fucking. fed. up. of. fucking. bumps.

system-f/Substitution.v
@@ -3,7 +3,7 @@
     single one. *)
 
 Require Export Syntax.
-Require Export Arith.
+Require Export ZArith.
 Open Scope t_scope.
 Open Scope list_scope.
 
@@ -16,11 +16,28 @@ Reserved Notation " [ γ ! n ] t " (at level 5).
 (* “bump k A” increments all except the first k free vars in A *)
 (* variants for type/term vars in types/terms *)
 
+Ltac order_cases := repeat (simpl ; 
+  match goal with 
+    | [ |- context[ lt_dec ?n1 ?n2 ]] => 
+        destruct (lt_dec n1 n2); try (exfalso; omega) 
+    | [ |- context[ eq_nat_dec ?n1 ?n2 ]] => 
+        destruct (eq_nat_dec n1 n2); try (exfalso; omega) 
+    | _ => auto 
+  end).
+
+
+
 Fixpoint ty_bump_ty (k:nat) (A:ty) :=
   match A with
     | ##n => if (lt_dec n k) then ##n else ##(S n)
     | A arrows B => (ty_bump_ty k A) arrows (ty_bump_ty k B)
     | allX, A => allX, (ty_bump_ty (S k) A)
+  end.
+
+Fixpoint ty_bumps_ty (k:nat) (A:ty) :=
+  match k with
+    | 0 => A
+    | S k' => ty_bump_ty 0 (ty_bumps_ty k' A)
   end.
 
 Fixpoint ty_bump_tm (k:nat) (t:tm) :=
@@ -32,6 +49,12 @@ Fixpoint ty_bump_tm (k:nat) (t:tm) :=
     | t0 @ A => (ty_bump_tm k t0) @ (ty_bump_ty k A)
   end.
 
+Fixpoint ty_bumps_tm (k:nat) (t:tm) :=
+  match k with
+    | 0 => t
+    | S k' => ty_bump_tm 0 (ty_bumps_tm k' t)
+  end.
+
 Fixpoint tm_bump_tm (k:nat) (t:tm) :=
   match t with
     | #n => if (lt_dec n k) then #n else #(S n)
@@ -41,15 +64,72 @@ Fixpoint tm_bump_tm (k:nat) (t:tm) :=
     | t0 @ A => (tm_bump_tm k t0) @ A
   end.
 
+Fixpoint tm_bumps_tm (k:nat) (t:tm) :=
+  match k with
+    | 0 => t
+    | S k' => tm_bump_tm 0 (tm_bumps_tm k' t)
+  end.
+
+Lemma ty_ty_bump_ty_commutes A : forall j k,
+  (ty_bump_ty (S (j+k)) (ty_bump_ty j A)) = (ty_bump_ty j (ty_bump_ty (j+k) A)).
+Proof. 
+  induction A as [ n | A IH0 B IH1 | A IH ]; intros; simpl.
+    order_cases. 
+    rewrite IH0; rewrite IH1; auto.
+    set (H := IH (S j) k); simpl in H; rewrite H.  auto.
+Qed.
+
+Lemma ty_ty_bump_tm_commutes t : forall j k,
+  (ty_bump_tm (S (j+k)) (ty_bump_tm j t)) = (ty_bump_tm j (ty_bump_tm (j+k) t)).
+Proof. 
+  induction t as [ n | A t0 IH | t0 IH0 t1 IH1 | t0 IH | t0 IH A]; intros; 
+    simpl.
+    order_cases.
+    rewrite IH.  rewrite ty_ty_bump_ty_commutes; simpl.  auto.
+    rewrite IH0; rewrite IH1; auto.
+    set (H := IH (S j) k); simpl in H; rewrite H; auto.
+    rewrite IH; rewrite ty_ty_bump_ty_commutes; auto.
+Qed.
+
+Lemma ty_tm_bump_commutes t : forall k j, 
+  ty_bump_tm k (tm_bump_tm j t) = tm_bump_tm j (ty_bump_tm k t).
+Proof. 
+  induction t as [ n | A t0 IH | t0 IH0 t1 IH1 | t0 IH | t0 IH A]; intros; 
+    simpl.
+      order_cases.
+      rewrite IH; auto.
+      rewrite IH0; rewrite IH1; auto.
+      rewrite IH; auto.
+      rewrite IH; auto.
+Qed.
+
+Lemma ty_tm_bump_bumps_commute t : forall j k,
+  ty_bump_tm k (tm_bumps_tm j t) = tm_bumps_tm j (ty_bump_tm k t).
+Proof.
+  induction j as [ | j' IH]; simpl.
+    auto.
+    intros.  rewrite ty_tm_bump_commutes.  rewrite IH.  auto.
+Qed.
+
+Lemma ty_tm_bumps_commute t : forall k j,
+  ty_bumps_tm k (tm_bumps_tm j t) = tm_bumps_tm j (ty_bumps_tm k t).
+Proof.
+  induction k as [ | k' IH]; simpl; intros.
+    auto.  
+    rewrite IH.  apply ty_tm_bump_bumps_commute.
+Qed.
+
+
+
 (* To understand the “unbumping” in substitution, think about how the variables of A, B (resp. s, t) should match up after an inst-reduction (resp. β-reduction) under a binder. *)
 
 (* Substitution of type A for index n in B *)
 Fixpoint ty_sub_ty A n B :=
   match B with
-    | ##k => if (eq_nat_dec k n) then A else
+    | ##k => if (eq_nat_dec k n) then (ty_bumps_ty n A) else
              if (lt_dec k n) then ##k else ##(pred k)
     | B0 arrows B1 => ([A /// n] B0) arrows ([A /// n] B1)
-    | allX, B0 => allX, [ty_bump_ty 0 A /// S n]B0
+    | allX, B0 => allX, [A /// S n]B0
   end
 where " [ A /// n ] B " := (ty_sub_ty A n B) : t_scope.
 
@@ -59,7 +139,7 @@ Fixpoint ty_sub_tm A n t :=
     | #k => #k
     | λx B, t0 => λx ([A /// n] B), [A // n] t0
     | t0 * t1 => [A//n]t0 * [A//n]t1
-    | ΛX, t0 => ΛX, [ty_bump_ty 0 A // S n] t0
+    | ΛX, t0 => ΛX, [A // S n] t0
     | t0 @ B => ([A // n] t0) @ ([A /// n] B)
   end
 where " [ A // n ] t " := (ty_sub_tm A n t) : t_scope.
@@ -68,14 +148,52 @@ where " [ A // n ] t " := (ty_sub_tm A n t) : t_scope.
 (* Substitution of term s for index n in t *)
 Fixpoint tm_sub_tm s n t :=
   match t with
-    | #k => if (eq_nat_dec k n) then s else
+    | #k => if (eq_nat_dec k n) then (tm_bumps_tm n s) else
              if (lt_dec k n) then #k else #(pred k)
-    | λx A, t0 => λx A, tm_sub_tm (tm_bump_tm 0 s) (S n) t0
-    | t0 * t1 => (tm_sub_tm s n t0) * (tm_sub_tm s n t1)
-    | ΛX, t0 => ΛX, (tm_sub_tm (ty_bump_tm 0 s) n t0)
+    | λx A, t0 => λx A, [s \ (S n)] t0
+    | t0 * t1 => [s\n]t0 * [s\n]t1
+    | ΛX, t0 => ΛX, [ (ty_bump_tm 0 s) \ n ] t0
     | t0 @ B => ([s \ n] t0) @ B
   end
 where " [ s \ n ] t " := (tm_sub_tm s n t) : t_scope.
+
+Lemma sub_closed_trivial : forall s n t, closed n t -> [s\n]t = t.
+Proof.
+  intros s n t; generalize dependent n.  generalize dependent s.
+  induction t as [ k | A t0 IH | t0 IH0 t1 IH1 | t0 IH | t0 IH A]; simpl; intros.
+  (* Case #k *) destruct (eq_nat_dec k n).  exfalso; omega.  destruct (lt_dec k n).  reflexivity.  exfalso; omega.
+  (* Case λx A, t0 *)  rewrite IH; auto.
+  (* Case t0 * t1 *) rewrite IH0; try tauto.  rewrite IH1; tauto.
+  (* Case ΛX, t0 *) rewrite IH; auto.
+  (* Case t0 @ A *) rewrite IH; auto.
+Qed.
+
+Lemma sub_bump_trivial : forall s n t, [s\n](tm_bump_tm n t) = t.
+Proof.
+  intros s n t.  generalize dependent n.  generalize dependent s.
+  induction t as [ k | A t0 IH | t0 IH0 t1 IH1 | t0 IH | t0 IH A]; simpl; intros.
+  (* Case #k *)
+  destruct (eq_nat_dec k n) as [ekn|nekn] _eqn; simpl;
+  destruct (lt_dec k n) as [lkn|gekn] _eqn; try (exfalso; omega); subst.
+     unfold tm_sub_tm.  destruct (eq_nat_dec (S n) n); destruct (lt_dec (S n) n); try (exfalso; omega).  auto.
+     unfold tm_sub_tm.  rewrite Heqs0.  rewrite Heqs1.  auto.
+     unfold tm_sub_tm.  destruct (eq_nat_dec (S k) n); destruct (lt_dec (S k) n); try (exfalso; omega).  auto.
+  (* Case λx A, t0 *)  rewrite IH; auto.
+  (* Case t0 * t1 *) rewrite IH0; try tauto.  rewrite IH1; tauto.
+  (* Case ΛX, t0 *) rewrite IH; auto.
+  (* Case t0 @ A *) rewrite IH; auto.
+Qed.
+
+Lemma ty_bump_in_tm_sub : forall t j k s,
+  ty_bump_tm j [s\k]t = [(ty_bump_tm j s)\k](ty_bump_tm j t).
+Proof.
+  induction t as [ n | A t0 IH | t0 IH0 t1 IH1 | t0 IH | t0 IH A]; simpl; intros.
+  (* Case #k *)  order_cases.  apply ty_tm_bump_bumps_commute.
+  (* Case λx A, t0 *)  rewrite IH; auto.
+  (* Case t0 * t1 *) rewrite IH0; try tauto.  rewrite IH1; tauto.
+  (* Case ΛX, t0 *) rewrite IH; rewrite (ty_ty_bump_tm_commutes _ 0 j); auto.
+  (* Case t0 @ A *) rewrite IH; auto.
+Qed.
 
 (* Substitution for the list γ, starting from index n in M *)
 (* Not — *not* simultaneous; done in order. *)
@@ -87,21 +205,71 @@ Fixpoint list_sub_tm (γ : list tm) (n : nat) (t : tm) :=
 where " [ γ ! n ] t " := (list_sub_tm γ n t) : t_scope.
 
 Lemma list_sub_lam γ : forall n A t,
-  [γ!n](λx A, t) = (λx A, [(List.map (tm_bump_tm 0) γ)!(S n)]t).
+  [γ!n](λx A, t) = (λx A, [γ!(S n)]t).
 Proof.
   induction γ as [ | s γ' IH]; intros.
   (* Case γ = nil *) auto.
   (* Case γ = s :: γ' *) simpl. apply IH.
 Qed.
 
-(*
+Lemma 
+Lemma tm_bump_in_sub : forall t s j k,
+  tm_bump_tm k [s\k+j]t = [s\(S (k+j))] (tm_bump_tm k t).
+Proof.
+  induction t as [ n | A t0 IH | t0 IH0 t1 IH1 | t0 IH | t0 IH A];
+    intros s j k.
+  (* SCase t = #k *) info order_cases.  destruct n; try (exfalso; omega); tauto.
+  (* SCase t = λx A, t0 *)
+    simpl.  rewrite IH.  auto.
+    simpl.  set (H := IH v w (S n)).  simpl in H.  rewrite H.  auto.
+  (* SCase t = t0 * t1 *)
+    simpl.  rewrite IH0.  rewrite IH1.  auto.
+  (* SCase t = ΛX, t0 *)
+    simpl.  rewrite <- IH.  rewrite H. auto.
+  (* SCase t = t0 @ A *)
+Lemma tm_bump_in_sub : forall t s j k,
+  tm_bumps_tm (j) [s\k]t = [s\j+k] (tm_bump_tm n w).
+Proof.
+
+
+Lemma adj_subs_commute : forall t v w n,
+  ([[v\0]w\n] [v\(S n)] t)
+  = [v\n][w\n] t.
+Proof.
+  induction t as [ k | A t0 IH | t0 IH0 t1 IH1 | t0 IH | t0 IH A];
+    intros v w n.
+  (* SCase t = #k *) order_cases.
+    apply tm_
+  (* SCase t = λx A, t0 *)
+    simpl.  set (H := IH v w (S n)).  simpl in H.  rewrite H.  auto.
+  (* SCase t = t0 * t1 *)
+    simpl.  rewrite IH0.  rewrite IH1.  auto.
+  (* SCase t = ΛX, t0 *)
+    simpl.  rewrite <- IH.  rewrite H. auto.
+  (* SCase t = t0 @ A *)
+
+
 Lemma list_sub_commute : forall γ t w,
-  ([w\0] [List.map (tm_bump_tm 0) γ ! 1] t)
-  = [ ([γ!0]w :: γ) ! 0 ] t.
+  ([[γ!0]w\0] [List.map (tm_bump_tm 0) γ ! 1] t)
+  = [ (w :: γ) ! 0 ] t.
 Proof.
   induction γ as [ | s γ' IHγ'].
-  (* case γ = nil *)  reflexivity.
-  (* case γ = s :: γ' *) induction t as [ n | A t IH | t0 IH0 t1 IH1 | t IH | t IH A]; simpl.
+  (* Case γ = nil *)
+    reflexivity.
+  (* Case γ = s :: γ' *) 
+    induction t as [ k | A t0 IH | t0 IH0 t1 IH1 | t0 IH | t0 IH A];
+      intros w.
+    (* SCase t = #k *)  simpl.  rewrite IHγ'.
+      destruct k as [ | [ | n'']]; simpl.
+        auto.
+        rewrite (sub_bump_trivial _ 0 s).  auto.
+        auto.
+    (* SCase t = λx A, t0 *)
+      rewrite IHγ'.
+    (* SCase t = t0 * t1 *)
+    (* SCase t = ΛX, t0 *)
+    (* SCase t = t0 @ A *)
+
 *)
 
 
